hax: Use hax_helper instead of anyhow closure. Extract all of primitives

securedrop-protocol/protocol-minimal/src/lib.rs
@@ -50,3 +50,5 @@ pub mod storage;
 pub mod encrypt_decrypt;
 pub mod message;
 pub mod metadata;
+
+pub mod hax_helper;
