securedrop-protocol/protocol-minimal/src/primitives/dh_akem.rs
@@ -1,6 +1,9 @@
+use anyhow::anyhow;
 use hpke_rs::{HpkePrivateKey, HpkePublicKey};
 use libcrux_kem::{PrivateKey, PublicKey};
 use rand_core::{CryptoRng, RngCore};
+
+use crate::hax_helper::HaxHelper;
 
 // todo: deprecate all this
 
@@ -132,12 +135,12 @@ fn typed(
     let private_key = DhAkemPrivateKey::from_bytes(
         private_key_bytes
             .try_into()
-            .map_err(|_| anyhow::anyhow!("Failed to convert private key bytes"))?,
+            .ok_or_err("Failed to convert private key bytes")?,
     );
     let public_key = DhAkemPublicKey::from_bytes(
         public_key_bytes
             .try_into()
-            .map_err(|_| anyhow::anyhow!("Failed to convert public key bytes"))?,
+            .ok_or_err("Failed to convert public key bytes")?,
     );
 
     Ok((private_key, public_key))
