securedrop-protocol/protocol-minimal/src/primitives/mlkem.rs
@@ -1,3 +1,4 @@
+use crate::hax_helper::HaxHelper;
 use libcrux_kem::{PrivateKey, PublicKey};
 use libcrux_ml_kem::{KEY_GENERATION_SEED_SIZE, mlkem768};
 use rand_core::{CryptoRng, RngCore};
@@ -105,12 +106,12 @@ fn typed(
     let private_key = MLKEM768PrivateKey::from_bytes(
         private_key_bytes
             .try_into()
-            .map_err(|_| anyhow::anyhow!("Failed to convert private key bytes"))?,
+            .ok_or_err("Failed to convert private key bytes")?,
     );
     let public_key = MLKEM768PublicKey::from_bytes(
         public_key_bytes
             .try_into()
-            .map_err(|_| anyhow::anyhow!("Failed to convert public key bytes"))?,
+            .ok_or_err("Failed to convert public key bytes")?,
     );
 
     Ok((private_key, public_key))
