securedrop-protocol/protocol-minimal/proofs/fstar/extraction/Securedrop_protocol_minimal.Hax_helper.fst
@@ -1,0 +1,74 @@
+module Securedrop_protocol_minimal.Hax_helper
+#set-options "--fuel 0 --ifuel 1 --z3rlimit 15"
+open FStar.Mul
+open Core_models
+
+let _ =
+  (* This module has implicit dependencies, here we make them explicit. *)
+  (* The implicit dependencies arise from typeclasses instances. *)
+  let open Anyhow.Kind in
+  ()
+
+/// do_something().map_err(|_| anyhow!("error_msg")) breaks hax.
+class t_HaxHelper (v_Self: Type0) (v_T: Type0) (v_E: Type0) = {
+  f_ok_or_err_pre:v_Self -> string -> Type0;
+  f_ok_or_err_post:v_Self -> string -> Core_models.Result.t_Result v_T Anyhow.t_Error -> Type0;
+  f_ok_or_err:x0: v_Self -> x1: string
+    -> Prims.Pure (Core_models.Result.t_Result v_T Anyhow.t_Error)
+        (f_ok_or_err_pre x0 x1)
+        (fun result -> f_ok_or_err_post x0 x1 result);
+  f_err_pre:v_Self -> string -> Type0;
+  f_err_post:v_Self -> string -> Anyhow.t_Error -> Type0;
+  f_err:x0: v_Self -> x1: string
+    -> Prims.Pure Anyhow.t_Error (f_err_pre x0 x1) (fun result -> f_err_post x0 x1 result)
+}
+
+[@@ FStar.Tactics.Typeclasses.tcinstance]
+let impl (#v_T #v_E: Type0) : t_HaxHelper (Core_models.Result.t_Result v_T v_E) v_T v_E =
+  {
+    f_ok_or_err_pre = (fun (self: Core_models.Result.t_Result v_T v_E) (msg: string) -> true);
+    f_ok_or_err_post
+    =
+    (fun
+        (self: Core_models.Result.t_Result v_T v_E)
+        (msg: string)
+        (out: Core_models.Result.t_Result v_T Anyhow.t_Error)
+        ->
+        true);
+    f_ok_or_err
+    =
+    (fun (self: Core_models.Result.t_Result v_T v_E) (msg: string) ->
+        match self <: Core_models.Result.t_Result v_T v_E with
+        | Core_models.Result.Result_Ok v ->
+          Core_models.Result.Result_Ok v <: Core_models.Result.t_Result v_T Anyhow.t_Error
+        | Core_models.Result.Result_Err _ ->
+          let error:Anyhow.t_Error =
+            match msg <: string with
+            | error ->
+              Anyhow.Kind.impl_Adhoc__new #string
+                (Anyhow.Kind.f_anyhow_kind #string #FStar.Tactics.Typeclasses.solve error
+                  <:
+                  Anyhow.Kind.t_Adhoc)
+                error
+          in
+          Core_models.Result.Result_Err (Anyhow.__private.must_use error)
+          <:
+          Core_models.Result.t_Result v_T Anyhow.t_Error);
+    f_err_pre = (fun (self: Core_models.Result.t_Result v_T v_E) (msg: string) -> true);
+    f_err_post
+    =
+    (fun (self: Core_models.Result.t_Result v_T v_E) (msg: string) (out: Anyhow.t_Error) -> true);
+    f_err
+    =
+    fun (self: Core_models.Result.t_Result v_T v_E) (msg: string) ->
+      let error:Anyhow.t_Error =
+        match msg <: string with
+        | error ->
+          Anyhow.Kind.impl_Adhoc__new #string
+            (Anyhow.Kind.f_anyhow_kind #string #FStar.Tactics.Typeclasses.solve error
+              <:
+              Anyhow.Kind.t_Adhoc)
+            error
+      in
+      Anyhow.__private.must_use error
+  }
