securedrop-protocol/protocol-minimal/proofs/fstar/extraction/Securedrop_protocol_minimal.Keys.fst
@@ -1,0 +1,31 @@
+module Securedrop_protocol_minimal.Keys
+#set-options "--fuel 0 --ifuel 1 --z3rlimit 15"
+open FStar.Mul
+open Core_models
+
+/// Generic KeyPair
+type t_KeyPair (v_SK: Type0) (v_PK: Type0) = {
+  f_sk:v_SK;
+  f_pk:v_PK
+}
+
+/// The public keys that make up one ephemeral key bundle
+type t_KeyBundlePublic = {
+  f_apke_pk:Securedrop_protocol_minimal.Message.t_MessagePublicKey;
+  f_metadata_pk:Securedrop_protocol_minimal.Metadata.t_MetadataPublicKey
+}
+
+type t_MessageKeyBundle = {
+  f_apke:Securedrop_protocol_minimal.Message.t_MessageKeyPair;
+  f_metadata_kp:Securedrop_protocol_minimal.Metadata.t_MetadataKeyPair
+}
+
+type t_SignedLongtermPubKeyBytes =
+  | SignedLongtermPubKeyBytes : t_Array u8 (mk_usize 1248) -> t_SignedLongtermPubKeyBytes
+
+type t_SessionStorage = {
+  f_fpf_key:Core_models.Option.t_Option Securedrop_protocol_minimal.Sign.t_VerifyingKey;
+  f_nr_key:Core_models.Option.t_Option Securedrop_protocol_minimal.Sign.t_VerifyingKey;
+  f_fpf_signature:Core_models.Option.t_Option
+  (Securedrop_protocol_minimal.Sign.t_Signature Securedrop_protocol_minimal.Sign.t_FpfOnNewsroom)
+}
