securedrop-protocol/protocol-minimal/proofs/fstar/extraction/Securedrop_protocol_minimal.Primitives.Mlkem.fst
@@ -7,7 +7,9 @@ let _ =
   (* This module has implicit dependencies, here we make them explicit. *)
   (* The implicit dependencies arise from typeclasses instances. *)
   let open Libcrux_kem in
+  let open Libcrux_ml_kem.Types in
   let open Rand_core in
+  let open Securedrop_protocol_minimal.Hax_helper in
   ()
 
 let v_MLKEM768_PUBLIC_KEY_LEN: usize = mk_usize 1184
@@ -17,9 +19,29 @@ let v_MLKEM768_PRIVATE_KEY_LEN: usize = mk_usize 2400
 /// MLKEM-768 public key.
 type t_MLKEM768PublicKey = | MLKEM768PublicKey : t_Array u8 (mk_usize 1184) -> t_MLKEM768PublicKey
 
+[@@ FStar.Tactics.Typeclasses.tcinstance]
+assume
+val impl_2': Core_models.Fmt.t_Debug t_MLKEM768PublicKey
+
+unfold
+let impl_2 = impl_2'
+
+let impl_3: Core_models.Clone.t_Clone t_MLKEM768PublicKey =
+  { f_clone = (fun x -> x); f_clone_pre = (fun _ -> True); f_clone_post = (fun _ _ -> True) }
+
 /// MLKEM-768 private key.
 type t_MLKEM768PrivateKey =
   | MLKEM768PrivateKey : t_Array u8 (mk_usize 2400) -> t_MLKEM768PrivateKey
+
+[@@ FStar.Tactics.Typeclasses.tcinstance]
+assume
+val impl_4': Core_models.Fmt.t_Debug t_MLKEM768PrivateKey
+
+unfold
+let impl_4 = impl_4'
+
+let impl_5: Core_models.Clone.t_Clone t_MLKEM768PrivateKey =
+  { f_clone = (fun x -> x); f_clone_pre = (fun _ -> True); f_clone_post = (fun _ _ -> True) }
 
 let impl_MLKEM768PublicKey__as_bytes (self: t_MLKEM768PublicKey) : t_Array u8 (mk_usize 1184) =
   self._0
@@ -32,6 +54,40 @@ let impl_MLKEM768PrivateKey__as_bytes (self: t_MLKEM768PrivateKey) : t_Array u8 
 
 let impl_MLKEM768PrivateKey__from_bytes (bytes: t_Array u8 (mk_usize 2400)) : t_MLKEM768PrivateKey =
   MLKEM768PrivateKey bytes <: t_MLKEM768PrivateKey
+
+let from_bytes (seed: t_Array u8 (mk_usize 64))
+    : Core_models.Result.t_Result (t_MLKEM768PrivateKey & t_MLKEM768PublicKey) Anyhow.t_Error =
+  let
+  (sk: Libcrux_ml_kem.Types.t_MlKemPrivateKey (mk_usize 2400)),
+  (pk: Libcrux_ml_kem.Types.t_MlKemPublicKey (mk_usize 1184)) =
+    Libcrux_ml_kem.Types.impl_24__into_parts (mk_usize 2400)
+      (mk_usize 1184)
+      (Libcrux_ml_kem.Mlkem768.generate_key_pair seed
+        <:
+        Libcrux_ml_kem.Types.t_MlKemKeyPair (mk_usize 2400) (mk_usize 1184))
+  in
+  let mlkem_encaps:t_MLKEM768PublicKey =
+    impl_MLKEM768PublicKey__from_bytes (Core_models.Convert.f_into #(Libcrux_ml_kem.Types.t_MlKemPublicKey
+            (mk_usize 1184))
+          #(t_Array u8 (mk_usize 1184))
+          #FStar.Tactics.Typeclasses.solve
+          pk
+        <:
+        t_Array u8 (mk_usize 1184))
+  in
+  let mlkem_decaps:t_MLKEM768PrivateKey =
+    impl_MLKEM768PrivateKey__from_bytes (Core_models.Convert.f_into #(Libcrux_ml_kem.Types.t_MlKemPrivateKey
+            (mk_usize 2400))
+          #(t_Array u8 (mk_usize 2400))
+          #FStar.Tactics.Typeclasses.solve
+          sk
+        <:
+        t_Array u8 (mk_usize 2400))
+  in
+  Core_models.Result.Result_Ok
+  (mlkem_decaps, mlkem_encaps <: (t_MLKEM768PrivateKey & t_MLKEM768PublicKey))
+  <:
+  Core_models.Result.t_Result (t_MLKEM768PrivateKey & t_MLKEM768PublicKey) Anyhow.t_Error
 
 /// Helper, convert libcrux type to our key types
 let typed (sk: Libcrux_kem.t_PrivateKey) (pk: Libcrux_kem.t_PublicKey)
@@ -107,9 +163,11 @@ let typed (sk: Libcrux_kem.t_PrivateKey) (pk: Libcrux_kem.t_PublicKey)
     Core_models.Result.t_Result (t_MLKEM768PrivateKey & t_MLKEM768PublicKey) Anyhow.t_Error
   else
     match
-      Core_models.Result.impl__map_err #(t_Array u8 (mk_usize 2400))
+      Securedrop_protocol_minimal.Hax_helper.f_ok_or_err #(Core_models.Result.t_Result
+            (t_Array u8 (mk_usize 2400)) (Alloc.Vec.t_Vec u8 Alloc.Alloc.t_Global))
+        #(t_Array u8 (mk_usize 2400))
         #(Alloc.Vec.t_Vec u8 Alloc.Alloc.t_Global)
-        #Anyhow.t_Error
+        #FStar.Tactics.Typeclasses.solve
         (Core_models.Convert.f_try_into #(Alloc.Vec.t_Vec u8 Alloc.Alloc.t_Global)
             #(t_Array u8 (mk_usize 2400))
             #FStar.Tactics.Typeclasses.solve
@@ -117,26 +175,18 @@ let typed (sk: Libcrux_kem.t_PrivateKey) (pk: Libcrux_kem.t_PublicKey)
           <:
           Core_models.Result.t_Result (t_Array u8 (mk_usize 2400))
             (Alloc.Vec.t_Vec u8 Alloc.Alloc.t_Global))
-        (fun temp_0_ ->
-            let _:Alloc.Vec.t_Vec u8 Alloc.Alloc.t_Global = temp_0_ in
-            let error:Anyhow.t_Error =
-              Anyhow.__private.format_err (Core_models.Fmt.Rt.impl_1__new_const (mk_usize 1)
-                    (let list = ["Failed to convert private key bytes"] in
-                      FStar.Pervasives.assert_norm (Prims.eq2 (List.Tot.length list) 1);
-                      Rust_primitives.Hax.array_of_list 1 list)
-                  <:
-                  Core_models.Fmt.t_Arguments)
-            in
-            Anyhow.__private.must_use error)
+        "Failed to convert private key bytes"
       <:
       Core_models.Result.t_Result (t_Array u8 (mk_usize 2400)) Anyhow.t_Error
     with
     | Core_models.Result.Result_Ok hoist7 ->
       let private_key:t_MLKEM768PrivateKey = impl_MLKEM768PrivateKey__from_bytes hoist7 in
       (match
-          Core_models.Result.impl__map_err #(t_Array u8 (mk_usize 1184))
+          Securedrop_protocol_minimal.Hax_helper.f_ok_or_err #(Core_models.Result.t_Result
+                (t_Array u8 (mk_usize 1184)) (Alloc.Vec.t_Vec u8 Alloc.Alloc.t_Global))
+            #(t_Array u8 (mk_usize 1184))
             #(Alloc.Vec.t_Vec u8 Alloc.Alloc.t_Global)
-            #Anyhow.t_Error
+            #FStar.Tactics.Typeclasses.solve
             (Core_models.Convert.f_try_into #(Alloc.Vec.t_Vec u8 Alloc.Alloc.t_Global)
                 #(t_Array u8 (mk_usize 1184))
                 #FStar.Tactics.Typeclasses.solve
@@ -144,17 +194,7 @@ let typed (sk: Libcrux_kem.t_PrivateKey) (pk: Libcrux_kem.t_PublicKey)
               <:
               Core_models.Result.t_Result (t_Array u8 (mk_usize 1184))
                 (Alloc.Vec.t_Vec u8 Alloc.Alloc.t_Global))
-            (fun temp_0_ ->
-                let _:Alloc.Vec.t_Vec u8 Alloc.Alloc.t_Global = temp_0_ in
-                let error:Anyhow.t_Error =
-                  Anyhow.__private.format_err (Core_models.Fmt.Rt.impl_1__new_const (mk_usize 1)
-                        (let list = ["Failed to convert public key bytes"] in
-                          FStar.Pervasives.assert_norm (Prims.eq2 (List.Tot.length list) 1);
-                          Rust_primitives.Hax.array_of_list 1 list)
-                      <:
-                      Core_models.Fmt.t_Arguments)
-                in
-                Anyhow.__private.must_use error)
+            "Failed to convert public key bytes"
           <:
           Core_models.Result.t_Result (t_Array u8 (mk_usize 1184)) Anyhow.t_Error
         with
